examples/iso_dh/DY.Example.DH.Protocol.Stateful.Proof.fst
@@ -90,13 +90,13 @@ let dh_event_pred: event_predicate dh_event =
 let all_sessions = [
   pki_tag_and_invariant;
   private_keys_tag_and_invariant;
-  (|local_state_dh_session.tag, local_state_predicate_to_local_bytes_state_predicate dh_session_pred|);
+  mk_local_state_tag_and_pred dh_session_pred;
 ]
 
 /// List of all local event predicates.
 
 let all_events = [
-  (dh_event_instance.tag, compile_event_pred dh_event_pred)
+  mk_event_tag_and_pred dh_event_pred;
 ]
 
 /// Create the global trace invariants.
@@ -113,39 +113,8 @@ instance dh_protocol_invs: protocol_invariants = {
 
 /// Lemmas that the global state predicate contains all the local ones
 
-// Below, the `has_..._predicate` are called with the implicit argument `#dh_protocol_invs`.
-// This argument could be omitted as it can be instantiated automatically by F*'s typeclass resolution algorithm.
-// However we instantiate it explicitly here so that the meaning of `has_..._predicate` is easier to understand.
-
-val all_sessions_has_all_sessions: unit -> Lemma (norm [delta_only [`%all_sessions; `%for_allP]; iota; zeta] (for_allP (has_local_bytes_state_predicate #dh_protocol_invs) all_sessions))
-let all_sessions_has_all_sessions () =
-  assert_norm(List.Tot.no_repeats_p (List.Tot.map dfst (all_sessions)));
-  mk_state_pred_correct #dh_protocol_invs all_sessions;
-  norm_spec [delta_only [`%all_sessions; `%for_allP]; iota; zeta] (for_allP (has_local_bytes_state_predicate #dh_protocol_invs) all_sessions)
-
-val full_dh_session_pred_has_pki_invariant: squash (has_pki_invariant #dh_protocol_invs)
-let full_dh_session_pred_has_pki_invariant = all_sessions_has_all_sessions ()
-
-val full_dh_session_pred_has_private_keys_invariant: squash (has_private_keys_invariant #dh_protocol_invs)
-let full_dh_session_pred_has_private_keys_invariant = all_sessions_has_all_sessions ()
-
-// As an example, below `#dh_protocol_invs` is omitted and instantiated using F*'s typeclass resolution algorithm
-val full_dh_session_pred_has_dh_invariant: squash (has_local_state_predicate dh_session_pred)
-let full_dh_session_pred_has_dh_invariant = all_sessions_has_all_sessions ()
-
-/// Lemmas that the global event predicate contains all the local ones
-
-val all_events_has_all_events: unit -> Lemma (norm [delta_only [`%all_events; `%for_allP]; iota; zeta] (for_allP (has_compiled_event_pred #dh_protocol_invs) all_events))
-let all_events_has_all_events () =
-  assert_norm(List.Tot.no_repeats_p (List.Tot.map fst (all_events)));
-  mk_event_pred_correct #dh_protocol_invs all_events;
-  norm_spec [delta_only [`%all_events; `%for_allP]; iota; zeta] (for_allP (has_compiled_event_pred #dh_protocol_invs) all_events);
-  let dumb_lemma (x:prop) (y:prop): Lemma (requires x /\ x == y) (ensures y) = () in
-  dumb_lemma (for_allP (has_compiled_event_pred #dh_protocol_invs) all_events) (norm [delta_only [`%all_events; `%for_allP]; iota; zeta] (for_allP (has_compiled_event_pred #dh_protocol_invs) all_events))
-
-// As an example, below `#dh_protocol_invs` is omitted and instantiated using F*'s typeclass resolution algorithm
-val full_dh_event_pred_has_dh_invariant: squash (has_event_pred dh_event_pred)
-let full_dh_event_pred_has_dh_invariant = all_events_has_all_events ()
+let _ = do_boilerplate mk_state_pred_correct all_sessions
+let _ = do_boilerplate mk_event_pred_correct all_events
 
 (*** Proofs ****)
 
